examples/ConcurrentMap/Impl.i.dfy
@@ -1,0 +1,55 @@
+include "PseudoCivl.dfy"
+include "ConcurrentLinearHashTable.i.dfy"
+
+module Impl {
+  import opened PseudoCivl
+  import L = LocalConcurrentLinearHashTable
+  import ConcurrentMap
+
+  type SharedState = seq<Mutex<L.Item>>
+  type ThreadState = L.ThreadState
+
+  type Key = ConcurrentMap.Key
+  type Value = ConcurrentMap.Value
+
+  method query(s: SharedState, key: Key, shared tid: Tid, linear r: RightPhase)
+  returns (res: Value, linear l: LeftPhase)
+  requires |s| > 0
+  {
+    var slot := L.SlotForKey(|s|, key);
+    res, l := query_loop(s, key, slot, tid, r);
+  }
+
+  method query_loop(s: SharedState, key: Key, slot: L.Slot, shared tid: Tid, linear r: RightPhase)
+  returns (res: Value, linear l_out: LeftPhase)
+  requires 0 <= slot.slot <= |s|
+  {
+    if slot.slot == |s| {
+      assume false;
+    } else {
+      s[slot.slot].Acq(tid, r);
+
+      var entry := s[slot.slot].Read(tid);
+
+      linear var l := shift_phase(r);
+      s[slot.slot].Rel(tid, l);
+
+      if entry.Empty? {
+        assume false;
+        l_out := l;
+      } else if entry.key == key {
+        if entry.Tombstone? {
+          assume false;
+          l_out := l;
+        } else {
+          l_out := l;
+          res := entry.value;
+        }
+      } else {
+        var slot' := L.Slot(slot.slot + 1);
+        linear var r' := do_yield(l);
+        res, l_out := query_loop(s, key, slot', tid, r');
+      }
+    }
+  }
+}
