examples/ConcurrentMap/PseudoCivl.dfy
@@ -1,0 +1,92 @@
+include "../../lib/Base/Option.s.dfy"
+
+/*module PseudoCivl {
+  class Env {
+    method do_yield()
+    modifies this
+  }
+
+  class Mutex<V> {
+    function has() 
+  }
+}*/
+
+module PseudoCivl {
+  import opened Options
+
+  linear datatype RightPhase = RightPhase // TODO make opaque
+  linear datatype LeftPhase = LeftPhase // TODO make opaque
+  linear datatype Tid = Tid // TODO make opaque
+
+  class Mutex<V> {
+    function {:axiom} lock() : Option<Tid>
+    reads this
+
+    function {:axiom} value() : V
+    reads this
+
+    // right-mover
+    method {:axiom} Acq(shared tid:Tid, shared r:RightPhase)
+    modifies this
+    ensures old(lock()) == None
+    ensures lock() == Some(tid)
+
+    // left-mover
+    method {:axiom} Rel(shared tid:Tid, shared l:LeftPhase)
+    modifies this
+    requires lock() == Some(tid)
+    ensures lock() == None
+
+    method {:axiom} Read(shared tid:Tid) returns (v: V)
+    requires lock() == Some(tid)
+    ensures v == value()
+
+    method {:axiom} Write(shared tid:Tid, v: V)
+    modifies this
+    requires lock() == Some(tid)
+    ensures v == value()
+  }
+
+  function arbitrary_objects(): set<object>
+
+  method do_yield(linear l:LeftPhase)
+  returns (linear r:RightPhase)
+  modifies arbitrary_objects()
+  //modifies all Mutex objects / all objects? // ?
+  //modifies *
+
+  method shift_phase(linear r:RightPhase)
+  returns (linear l:LeftPhase)
+}
+
+/*module ExampleUsage {
+  method stuff(m: Mutex<int>, linear tid: TID, linear r:RightPhase) {
+    {
+      m.Acq(tid, r)
+      var l := shift_phase(r);
+      m.Rel(tid, l)
+    }
+
+    r := yield(l);
+
+    {
+      m.Acq(tid, r)
+      var l := shift_phase(r);
+      m.Rel(tid, l)
+    }
+  }
+
+  function I(s: seq<Entry>) : LocalConcurrentLinearHashTable.SharedVariables
+
+  method LockAdvance(s: seq<Entry>, linear tid: TID, localThreadState: LocalThreadState)
+  ensures LocalConcurrentLinearHashTable.InsertAdvance(old(I(s)), old(localThreadState), I(s), localThreadState)
+  {
+    s[localThreadState.currentSlot].Acquire();
+
+    // do some work with s[i]
+
+    s[localThreadState.currentSlot].Release();
+
+    localThreadState.currentSlot += 1;
+  }
+}*/
